theories/MP/GLTraceEquiv.v
@@ -1,0 +1,31 @@
+From mathcomp.ssreflect Require Import all_ssreflect seq.
+From mathcomp Require Import finmap.
+Set Implicit Arguments.
+Unset Strict Implicit.
+Import Prenex Implicits.
+
+Require Import MPST.MP.Atom.
+Require Import MPST.MP.Role.
+Require Import MPST.MP.Forall.
+Require Import MPST.MP.LNVar.
+Require Import MPST.MP.Global.
+Require Import MPST.MP.Local.
+Require Import MPST.MP.Actions.
+Require Import MPST.MP.Projection.
+
+Section TraceEquiv.
+
+  Definition step_equiv G P :=
+    forall a, exists G' P', step a G G' <-> lstep a P P'.
+
+  Definition trace_equiv G P :=
+    forall a, exists G' P', g_lts a G G' <-> l_lts a P P'.
+
+  Theorem global_local_trequiv G :
+    forall P,
+    projection G == Some P ->
+    trace_equiv (init G) ([::], P).
+  Proof.
+  Admitted.
+
+End TraceEquiv.
